theories/Simple.v
@@ -7,20 +7,28 @@ From Coq Require Import
 
 From ITree Require
      Core.ITree
-     Eq.UpToTaus.
+     Eq.UpToTaus
+     Interp.Interp.
 
 From ITree Require Import
+     Basics.Basics
      Eq.Shallow.
 
 Set Primitive Projections.
 (* end hide *)
 
-(** This is implemented by the (opaque) module
-    [ITree.Simple.Simple]. *)
 Module Type SimpleInterface.
+(** This interface is implemented by the module
+    [ITree.Simple.Simple]. *)
 
 (** ** Core definitions *)
+
 Include ITree.Core.ITree.
+Import ITreeNotations.
+
+Include ITree.Interp.Interp.
+
+Include ITree.Indexed.Sum.
 
 (** ** Equational theory *)
 
@@ -34,14 +42,16 @@ Parameter eutt : itree E R -> itree E R -> Prop.
 
 Infix "≈" := eutt (at level 40).
 
+(** [eutt] is an equivalence relation. *)
 Global Declare Instance Equivalence_eutt :
     Equivalence eutt.
 
+(** We can erase taus unter [eutt]. *)
+Parameter eutt_tau : forall (t : itree E R),
+    Tau t ≈ t.
+
 Parameter itree_eta : forall (t : itree E R),
     t ≈ go (observe t).
-
-Parameter tau_eutt : forall (t : itree E R),
-    Tau t ≈ t.
 
 Parameter eutt_ret : forall (r1 r2 : R),
     r1 = r2 <-> Ret r1 ≈ Ret r2.
@@ -49,32 +59,20 @@ Parameter eutt_ret : forall (r1 r2 : R),
 Parameter eutt_vis : forall {U : Type} (e : E U) (k1 k2 : U -> itree E R),
     (forall u, k1 u ≈ k2 u) <-> Vis e k1 ≈ Vis e k2.
 
-Global Declare Instance eutt_go :
-  Proper (going eutt ==> eutt) (@go E R).
-
-Global Declare Instance eutt_observe :
-  Proper (eutt ==> going eutt) (@observe E R).
-
-Global Declare Instance eutt_TauF :
-  Proper (eutt ==> going eutt) (@TauF E R _).
-
-Global Declare Instance eutt_VisF {u} (e: E u) :
-  Proper (pointwise_relation _ eutt ==> going eutt) (VisF e).
-
 End General.
 
 Infix "≈" := eutt (at level 40).
+
+(** *** Rewriting lemmas *)
 
 Parameter unfold_bind
   : forall {E R S} (t : itree E R) (k : R -> itree E S),
     ITree.bind t k
   ≈ ITree._bind k (fun t => ITree.bind t k) (observe t).
 
+(** The next two are immediate corollaries of [unfold_bind]. *)
 Parameter ret_bind : forall {E R S} (r : R) (k : R -> itree E S),
     ITree.bind (Ret r) k ≈ k r.
-
-Parameter tau_bind : forall {E R} U t (k: U -> itree E R),
-    ITree.bind (Tau t) k ≈ Tau (ITree.bind t k).
 
 Parameter vis_bind
   : forall {E R} U V (e: E V) (ek: V -> itree E U) (k: U -> itree E R),
@@ -90,11 +88,64 @@ Parameter bind_bind
     ITree.bind (ITree.bind s k) h
   ≈ ITree.bind s (fun r => ITree.bind (k r) h).
 
+Parameter unfold_aloop
+  : forall {E A B} (f : A -> itree E A + B) (x : A),
+    ITree.aloop f x
+  ≈ ITree._aloop id (ITree.aloop f) (f x).
+
+Hint Rewrite @eutt_tau : itree.
 Hint Rewrite @ret_bind : itree.
 Hint Rewrite @tau_bind : itree.
 Hint Rewrite @vis_bind : itree.
 Hint Rewrite @bind_ret : itree.
 Hint Rewrite @bind_bind : itree.
+
+(** **** Interp *)
+
+Definition _interp {E F} (f : E ~> itree F) R (ot : itreeF E R _)
+  : itree F R
+  := match ot with
+     | RetF r => Ret r
+     | TauF t => Tau (interp f _ t)
+     | VisF e k => Tau (f _ e >>= (fun x => interp f _ (k x)))
+     end.
+
+Parameter unfold_interp
+  : forall {E F R} {f : E ~> itree F} (t : itree E R),
+    interp f _ t ≈ (_interp f _ (observe t)).
+
+(** The next three are immediate corollaries of [unfold_interp]. *)
+Parameter ret_interp
+  : forall {E F R} {f : E ~> itree F} (x: R),
+    interp f _ (Ret x) ≈ Ret x.
+
+Parameter vis_interp
+  : forall {E F R} {f : E ~> itree F} U (e: E U) (k: U -> itree E R),
+    interp f _ (Vis e k)
+  ≈ Tau (ITree.bind (f _ e) (fun x => interp f _ (k x))).
+
+Parameter interp_lift : forall {E F : Type -> Type} {R : Type}
+      (f : E ~> (itree F)) (e : E R),
+    interp f _ (ITree.lift e) ≈ f _ e.
+
+Parameter interp_bind : forall {E F R S}
+      (f : E ~> itree F) (t : itree E R) (k : R -> itree E S),
+    interp f _ (ITree.bind t k)
+  ≈ ITree.bind (interp f _ t) (fun r => interp f _ (k r)).
+
+(** *** [Proper] lemmas *)
+
+Declare Instance eutt_go {E R} :
+  Proper (going eutt ==> eutt) (@go E R).
+
+Declare Instance eutt_observe {E R} :
+  Proper (eutt ==> going eutt) (@observe E R).
+
+Declare Instance eutt_TauF {E R} :
+  Proper (eutt ==> going eutt) (@TauF E R _).
+
+Declare Instance eutt_VisF {E R X} (e: E X) :
+  Proper (pointwise_relation _ (@eutt E R) ==> going eutt) (VisF e).
 
 Declare Instance eutt_bind {E R S} :
   Proper (eutt ==> pointwise_relation _ eutt ==> eutt)
@@ -104,17 +155,15 @@ Declare Instance eutt_map {E R S} :
   Proper (pointwise_relation _ eq ==> eutt ==> eutt)
          (@ITree.map E R S).
 
-Parameter unfold_aloop
-  : forall {E A B} (f : A -> itree E A + B) (x : A),
-    ITree.aloop f x
-  ≈ ITree._aloop id (ITree.aloop f) (f x).
+Declare Instance eutt_interp (E F : Type -> Type) f (R : Type) :
+  Proper (eutt ==> eutt) (@interp E F f R).
 
 End SimpleInterface.
 
 (** * Implementation *)
 
 (* TODO: implement *)
-
+(*
 Module Import Simple : SimpleInterface.
 
 Include ITree.Core.ITree.
@@ -203,3 +252,4 @@ Parameter unfold_aloop
   ≈ ITree._aloop id (ITree.aloop f) (f x).
 
 End Simple.
+*)
